PartialMonotonicity.v
@@ -105,36 +105,10 @@ Module PartialMonotonicity.
   Hint Resolve partialMonotonicity_freshness: pM.
 
 
-
-  Definition partialMonotonicity_prop (k : nat) :=  forall (e: Expr) (σ σ': Store) (ρ: Env) (v v': Value),
-      ⟦e⟧(σ, ρ, v)(k) = (Success v' σ') -> σ ⪯ σ'.
-
-  Definition partialMonotonicity_prop_list n := (eval_list_prop partialMonotonicity n partialMonotonicity_reflexivity partialMonotonicity_transitivity).
-
-  Definition partialMonotonicity_prop_init n := (eval_init_prop partialMonotonicity n partialMonotonicity_reflexivity partialMonotonicity_transitivity partialMonotonicity_assignment).
-
-
-  Theorem partialMonotonicity_theorem: forall (n : nat), (partialMonotonicity_prop n).
+  Theorem partialMonotonicity_theorem: forall (n : nat), forall (e: Expr) (σ σ': Store) (ρ: Env) (v v': Value),
+      ⟦e⟧(σ, ρ, v)(n) = (Success v' σ') -> σ ⪯ σ'.
   Proof.
-    apply strong_induction. unfold partialMonotonicity_prop. intros n H_strong; intros.
-    (* To get one step of the evaluator, we destruct n *)
-    destruct n; unfold partialMonotonicity_prop => //. (* n = 0 is discarded automatically *)
-    (* n > 0 - case analysis over e *)
-    move : (PeanoNat.Nat.lt_succ_diag_r n) => Hn.
-    destruct e;
-      (* Trivial cases are handled automatically *)
-      repeat light || invert_constructor_equalities || destruct_match || eauto 3 with pM.
-    - (* case e = e0.m(ē) *)
-      apply (iff_sym (PeanoNat.Nat.le_succ_l n (S n))) in Hn.
-      pose proof (partialMonotonicity_prop_list (S n) H_strong n Hn _ _ _ _ _ _ matched3); eauto with pM.
-    - (* case e = new C(l) *)
-      apply (iff_sym (PeanoNat.Nat.le_succ_l n (S n))) in Hn.
-      pose proof (partialMonotonicity_prop_init (S n) H_strong n Hn _ _ _ _ _ matched0).
-      pose proof (partialMonotonicity_prop_list (S n) H_strong n Hn _ _ _ _ _ _ matched); eauto with pM.
-    - (* case e1.v0 = e2 ; e3 *)
-      apply (partialMonotonicity_transitivity σ s σ'); eauto.
-      apply (partialMonotonicity_transitivity s (assign v1 v0 v2 s0) σ'); eauto.
-      unfold assign. repeat destruct_match; eauto using PeanoNat.Nat.eq_le_incl, update_one3 with pM.
+    apply (eval_prop partialMonotonicity); unfold Reflexive, Transitive, Assignment, Freshness; eauto with pM.
   Qed.
 
 
